lib/monads: restyle Trace_Monad.thy
This should now be in sync with Nondet_Monad.thy wherever the two files
have similar content.

Signed-off-by: Corey Lewis <corey.lewis@proofcraft.systems>

lib/Monads/trace/Trace_Monad.thy
@@ -1,62 +1,60 @@
 (*
+ * Copyright 2023, Proofcraft Pty Ltd
  * Copyright 2020, Data61, CSIRO (ABN 41 687 119 230)
  *
  * SPDX-License-Identifier: BSD-2-Clause
  *)
+
+chapter "Interference Trace Monad"
+
 theory Trace_Monad
-imports
-  Monad_Lib
-  Strengthen
+  imports
+    Fun_Pred_Syntax
+    Monad_Lib
+    Strengthen
 begin
 
 text \<open>
-The ``Interference Trace Monad''. This nondeterministic monad
-records the state at every interference point, permitting
-nondeterministic interference by the environment at interference
-points.
+  The ``Interference Trace Monad''. This nondeterministic monad
+  records the state at every interference point, permitting
+  nondeterministic interference by the environment at these points.
 
-The trace set initially includes all possible environment behaviours.
-Trace steps are tagged as environment or self actions, and can then
-be constrained to a smaller set where the environment acts according
-to a rely constraint (i.e. rely-guarantee reasoning), or to set the
-environment actions to be the self actions of another program (parallel
-composition).
-\<close>
+  The trace set initially includes all possible environment behaviours.
+  Trace steps are tagged as environment or self actions, and can then
+  be constrained to a smaller set where the environment acts according
+  to a rely constraint (i.e. rely-guarantee reasoning), or to set the
+  environment actions to be the self actions of another program (parallel
+  composition).\<close>
 
 section "The Trace Monad"
 
 text \<open>Trace monad identifier. Me corresponds to the current thread running and Env to the environment.\<close>
 datatype tmid = Me | Env
 
-text \<open>Results associated with traces. Traces may correspond to incomplete, failed, or completed executions.\<close>
+text \<open>
+  Results associated with traces. Traces may correspond to incomplete, failed, or completed executions.\<close>
 datatype ('s, 'a) tmres = Failed | Incomplete | Result "('a \<times> 's)"
 
-abbreviation
-  map_tmres_rv :: "('a \<Rightarrow> 'b) \<Rightarrow> ('s, 'a) tmres \<Rightarrow> ('s, 'b) tmres"
-where
+abbreviation map_tmres_rv :: "('a \<Rightarrow> 'b) \<Rightarrow> ('s, 'a) tmres \<Rightarrow> ('s, 'b) tmres" where
   "map_tmres_rv f \<equiv> map_tmres id f"
 
 section "The Monad"
 
-text \<open> tmonad returns a set of non-deterministic  computations, including
+text \<open>
+  tmonad returns a set of non-deterministic  computations, including
   a trace as a list of "thread identifier" \<times> state, and an optional
-  pair result, state when the computation did not fail. \<close>
+  pair result, state when the computation did not fail.\<close>
 type_synonym ('s, 'a) tmonad = "'s \<Rightarrow> ((tmid \<times> 's) list \<times> ('s, 'a) tmres) set"
 
 text \<open>Returns monad results, ignoring failures and traces.\<close>
-definition
-  mres :: "((tmid \<times> 's) list \<times> ('s, 'a) tmres) set \<Rightarrow> ('a \<times> 's) set"
-where
+definition mres :: "((tmid \<times> 's) list \<times> ('s, 'a) tmres) set \<Rightarrow> ('a \<times> 's) set" where
   "mres r = Result -` (snd ` r)"
 
 text \<open>
   The definition of fundamental monad functions @{text return} and
   @{text bind}. The monad function @{text "return x"} does not change
-  the  state, does not fail, and returns @{text "x"}.
-\<close>
-definition
-  return :: "'a \<Rightarrow> ('s,'a) tmonad"
-where
+  the  state, does not fail, and returns @{text "x"}.\<close>
+definition return :: "'a \<Rightarrow> ('s,'a) tmonad" where
   "return a \<equiv> \<lambda>s. ({([], Result (a, s))})"
 
 text \<open>
@@ -67,58 +65,41 @@ text \<open>
   the combined operation is the union of the set of sets that is created
   by @{text g} applied to the result sets of @{text f}. The combined
   operation may have failed, if @{text f} may have failed or @{text g} may
-  have failed on any of the results of @{text f}.
-\<close>
-
-abbreviation (input)
-  fst_upd :: "('a \<Rightarrow> 'c) \<Rightarrow> 'a \<times> 'b \<Rightarrow> 'c \<times> 'b"
-where
+  have failed on any of the results of @{text f}.\<close>
+abbreviation (input) fst_upd :: "('a \<Rightarrow> 'c) \<Rightarrow> 'a \<times> 'b \<Rightarrow> 'c \<times> 'b" where
   "fst_upd f \<equiv> \<lambda>(a,b). (f a, b)"
 
-abbreviation (input)
-  snd_upd :: "('b \<Rightarrow> 'c) \<Rightarrow> 'a \<times> 'b \<Rightarrow> 'a \<times> 'c"
-where
+abbreviation (input) snd_upd :: "('b \<Rightarrow> 'c) \<Rightarrow> 'a \<times> 'b \<Rightarrow> 'a \<times> 'c" where
   "snd_upd f \<equiv> \<lambda>(a,b). (a, f b)"
 
-definition
-  bind :: "('s, 'a) tmonad \<Rightarrow> ('a \<Rightarrow> ('s, 'b) tmonad) \<Rightarrow>
-           ('s, 'b) tmonad" (infixl ">>=" 60)
-where
+definition bind ::
+  "('s, 'a) tmonad \<Rightarrow> ('a \<Rightarrow> ('s, 'b) tmonad) \<Rightarrow> ('s, 'b) tmonad" (infixl ">>=" 60)
+  where
   "bind f g \<equiv> \<lambda>s. \<Union>(xs, r) \<in> (f s). case r of Failed \<Rightarrow> {(xs, Failed)}
     | Incomplete \<Rightarrow> {(xs, Incomplete)}
     | Result (rv, s) \<Rightarrow> fst_upd (\<lambda>ys. ys @ xs) ` g rv s"
 
 text \<open>Sometimes it is convenient to write @{text bind} in reverse order.\<close>
-abbreviation(input)
-  bind_rev :: "('c \<Rightarrow> ('a, 'b) tmonad) \<Rightarrow> ('a, 'c) tmonad \<Rightarrow>
-               ('a, 'b) tmonad" (infixl "=<<" 60)
-where
+abbreviation(input) bind_rev ::
+  "('c \<Rightarrow> ('a, 'b) tmonad) \<Rightarrow> ('a, 'c) tmonad \<Rightarrow> ('a, 'b) tmonad" (infixl "=<<" 60)
+  where
   "g =<< f \<equiv> f >>= g"
 
 text \<open>
   The basic accessor functions of the state monad. @{text get} returns
   the current state as result, does not fail, and does not change the state.
   @{text "put s"} returns nothing (@{typ unit}), changes the current state
-  to @{text s} and does not fail.
-\<close>
-definition
-  get :: "('s,'s) tmonad"
-where
+  to @{text s} and does not fail.\<close>
+definition get :: "('s,'s) tmonad" where
   "get \<equiv> \<lambda>s. {([], Result (s, s))}"
 
-definition
-  put :: "'s \<Rightarrow> ('s, unit) tmonad"
-where
-  "put s \<equiv> \<lambda>st. {([], Result ((), s))}"
+definition put :: "'s \<Rightarrow> ('s, unit) tmonad" where
+  "put s \<equiv> \<lambda>_. {([], Result ((), s))}"
 
-definition
-  put_trace_elem :: "(tmid \<times> 's) \<Rightarrow> ('s, unit) tmonad"
-where
+definition put_trace_elem :: "(tmid \<times> 's) \<Rightarrow> ('s, unit) tmonad" where
   "put_trace_elem x = (\<lambda>s. {([], Incomplete), ([x], Result ((), s))})"
 
-primrec
-  put_trace :: "(tmid \<times> 's) list \<Rightarrow> ('s, unit) tmonad"
-where
+primrec put_trace :: "(tmid \<times> 's) list \<Rightarrow> ('s, unit) tmonad" where
     "put_trace [] = return ()"
   | "put_trace (x # xs) = (put_trace xs >>= (\<lambda>_. put_trace_elem x))"
 
@@ -129,154 +110,118 @@ text \<open>
   of the set @{text A}, does not change the state, and does not fail
   (even if the set is empty). @{text "f \<sqinter> g"} executes @{text f} or
   executes @{text g}. It retuns the union of results of @{text f} and
-  @{text g}, and may have failed if either may have failed.
-\<close>
-definition
-  select :: "'a set \<Rightarrow> ('s, 'a) tmonad"
-where
-  (* Should we have Failed when A = {} ? *)
+  @{text g}, and may have failed if either may have failed.\<close>
+definition select :: "'a set \<Rightarrow> ('s, 'a) tmonad" where
   "select A \<equiv> \<lambda>s. (Pair [] ` Result ` (A \<times> {s}))"
 
-definition
-  alternative :: "('s,'a) tmonad \<Rightarrow> ('s,'a) tmonad \<Rightarrow>
-                  ('s,'a) tmonad"
-  (infixl "\<sqinter>" 20)
-where
+definition alternative :: "('s,'a) tmonad \<Rightarrow> ('s,'a) tmonad \<Rightarrow> ('s,'a) tmonad"
+  (infixl "\<sqinter>" 20) where
   "f \<sqinter> g \<equiv> \<lambda>s. (f s \<union> g s)"
 
-
-text \<open> The @{text selet_f} function was left out here until we figure
-  out what variant we actually need.
-\<close>
+text \<open>
+  The @{text select_f} function was left out here until we figure
+  out what variant we actually need.\<close>
 
 subsection "Failure"
 
-text \<open> The monad function that always fails. Returns an empty set of
-results and sets the failure flag. \<close>
-definition
-  fail :: "('s, 'a) tmonad"
-where
- "fail \<equiv> \<lambda>s. {([], Failed)}"
+text \<open>
+  The monad function that always fails. Returns an empty set of results and sets the failure flag.\<close>
+definition fail :: "('s, 'a) tmonad" where
+  "fail \<equiv> \<lambda>s. {([], Failed)}"
 
-text \<open> Assertions: fail if the property @{text P} is not true \<close>
-definition
-  assert :: "bool \<Rightarrow> ('a, unit) tmonad"
-where
- "assert P \<equiv> if P then return () else fail"
+text \<open>Assertions: fail if the property @{text P} is not true\<close>
+definition assert :: "bool \<Rightarrow> ('a, unit) tmonad" where
+  "assert P \<equiv> if P then return () else fail"
 
-text \<open> Fail if the value is @{const None},
-  return result @{text v} for @{term "Some v"} \<close>
-definition
-  assert_opt :: "'a option \<Rightarrow> ('b, 'a) tmonad"
-where
- "assert_opt v \<equiv> case v of None \<Rightarrow> fail | Some v \<Rightarrow> return v"
+text \<open>Fail if the value is @{const None}, return result @{text v} for @{term "Some v"}\<close>
+definition assert_opt :: "'a option \<Rightarrow> ('b, 'a) tmonad" where
+  "assert_opt v \<equiv> case v of None \<Rightarrow> fail | Some v \<Rightarrow> return v"
 
-text \<open> An assertion that also can introspect the current state. \<close>
-
-definition
-  state_assert :: "('s \<Rightarrow> bool) \<Rightarrow> ('s, unit) tmonad"
-where
+text \<open>An assertion that also can introspect the current state.\<close>
+definition state_assert :: "('s \<Rightarrow> bool) \<Rightarrow> ('s, unit) tmonad" where
   "state_assert P \<equiv> get >>= (\<lambda>s. assert (P s))"
 
 subsection "Generic functions on top of the state monad"
 
-text \<open> Apply a function to the current state and return the result
-without changing the state. \<close>
-definition
-  gets :: "('s \<Rightarrow> 'a) \<Rightarrow> ('s, 'a) tmonad"
-where
- "gets f \<equiv> get >>= (\<lambda>s. return (f s))"
+text \<open>Apply a function to the current state and return the result without changing the state.\<close>
+definition gets :: "('s \<Rightarrow> 'a) \<Rightarrow> ('s, 'a) tmonad" where
+  "gets f \<equiv> get >>= (\<lambda>s. return (f s))"
 
-text \<open> Modify the current state using the function passed in. \<close>
-definition
-  modify :: "('s \<Rightarrow> 's) \<Rightarrow> ('s, unit) tmonad"
-where
+text \<open>Modify the current state using the function passed in.\<close>
+definition modify :: "('s \<Rightarrow> 's) \<Rightarrow> ('s, unit) tmonad" where
   "modify f \<equiv> get >>= (\<lambda>s. put (f s))"
 
-lemma simpler_gets_def: "gets f = (\<lambda>s. {([], Result ((f s), s))})"
- by (simp add: fun_eq_iff gets_def return_def bind_def get_def split_def)
+lemma simpler_gets_def:
+  "gets f = (\<lambda>s. {([], Result ((f s), s))})"
+  by (simp add: gets_def return_def bind_def get_def)
 
 lemma simpler_modify_def:
   "modify f = (\<lambda>s. {([], Result ((),(f s)))})"
-  by (simp add: fun_eq_iff modify_def bind_def get_def put_def split_def)
+  by (simp add: modify_def bind_def get_def put_def)
 
-text \<open> Execute the given monad when the condition is true,
-  return @{text "()"} otherwise. \<close>
-definition
-  "when" :: "bool \<Rightarrow> ('s, unit) tmonad \<Rightarrow>
-           ('s, unit) tmonad"
-where
+text \<open>Execute the given monad when the condition is true, return @{text "()"} otherwise.\<close>
+definition "when" :: "bool \<Rightarrow> ('s, unit) tmonad \<Rightarrow> ('s, unit) tmonad" where
   "when P m \<equiv> if P then m else return ()"
 
-text \<open> Execute the given monad unless the condition is true,
-  return @{text "()"} otherwise. \<close>
-definition
-  unless :: "bool \<Rightarrow> ('s, unit) tmonad \<Rightarrow>
-            ('s, unit) tmonad"
-where
+text \<open>Execute the given monad unless the condition is true, return @{text "()"} otherwise.\<close>
+definition unless :: "bool \<Rightarrow> ('s, unit) tmonad \<Rightarrow> ('s, unit) tmonad" where
   "unless P m \<equiv> when (\<not>P) m"
 
 text \<open>
   Perform a test on the current state, performing the left monad if
-  the result is true or the right monad if the result is false.
-\<close>
-definition
-  condition :: "('s \<Rightarrow> bool) \<Rightarrow> ('s, 'r) tmonad \<Rightarrow> ('s, 'r) tmonad \<Rightarrow> ('s, 'r) tmonad"
-where
+  the result is true or the right monad if the result is false.\<close>
+definition condition ::
+  "('s \<Rightarrow> bool) \<Rightarrow> ('s, 'r) tmonad \<Rightarrow> ('s, 'r) tmonad \<Rightarrow> ('s, 'r) tmonad" where
   "condition P L R \<equiv> \<lambda>s. if (P s) then (L s) else (R s)"
 
 notation (output)
   condition  ("(condition (_)//  (_)//  (_))" [1000,1000,1000] 1000)
 
 text \<open>
-Apply an option valued function to the current state, fail
-if it returns @{const None}, return @{text v} if it returns
-@{term "Some v"}.
-\<close>
-definition
-  gets_the :: "('s \<Rightarrow> 'a option) \<Rightarrow> ('s, 'a) tmonad"
-where
+  Apply an option valued function to the current state, fail if it returns @{const None},
+  return @{text v} if it returns @{term "Some v"}.\<close>
+definition gets_the :: "('s \<Rightarrow> 'a option) \<Rightarrow> ('s, 'a) tmonad" where
   "gets_the f \<equiv> gets f >>= assert_opt"
 
 
-subsection \<open> The Monad Laws \<close>
+subsection \<open>The Monad Laws\<close>
 
 text \<open>An alternative definition of bind, sometimes more convenient.\<close>
 lemma bind_def2:
-  "bind f g \<equiv> (\<lambda>s. ((\<lambda>xs. (xs, Failed)) ` {xs. (xs, Failed) \<in> f s})
-    \<union> ((\<lambda>xs. (xs, Incomplete)) ` {xs. (xs, Incomplete) \<in> f s})
-    \<union> (\<Union>(xs, rv, s) \<in> {(xs, rv, s'). (xs, Result (rv, s')) \<in> f s}. fst_upd (\<lambda>ys. ys @ xs) ` g rv s))"
+  "bind f g \<equiv>
+     \<lambda>s. ((\<lambda>xs. (xs, Failed)) ` {xs. (xs, Failed) \<in> f s})
+         \<union> ((\<lambda>xs. (xs, Incomplete)) ` {xs. (xs, Incomplete) \<in> f s})
+         \<union> (\<Union>(xs, rv, s) \<in> {(xs, rv, s'). (xs, Result (rv, s')) \<in> f s}. fst_upd (\<lambda>ys. ys @ xs) ` g rv s)"
   apply (clarsimp simp add: bind_def fun_eq_iff
                             Un_Union_image split_def
                     intro!: eq_reflection)
-  apply (auto split: tmres.splits elim!:rev_bexI[where A="f x" for x])
-  apply (fastforce intro: image_eqI[rotated])
+  apply (fastforce split: tmres.splits elim!: rev_bexI[where A="f x" for x]
+                   intro: image_eqI[rotated])
   done
 
 lemma elem_bindE:
-  "(tr, res) \<in> bind f (\<lambda>x. g x) s
-    \<Longrightarrow> ((res = Incomplete | res = Failed) \<Longrightarrow> (tr, map_tmres undefined undefined res) \<in> f s \<Longrightarrow> P)
-    \<Longrightarrow> (\<And>tr' tr'' x s'. (tr', Result (x, s')) \<in> f s \<Longrightarrow> (tr'', res) \<in> g x s'
-        \<Longrightarrow> tr = tr'' @ tr' \<Longrightarrow> P)
-    \<Longrightarrow> P"
+  "\<lbrakk>(tr, res) \<in> bind f g s;
+    \<lbrakk>res = Incomplete \<or> res = Failed; (tr, map_tmres undefined undefined res) \<in> f s\<rbrakk> \<Longrightarrow> P;
+    \<And>tr' tr'' x s'. \<lbrakk>(tr', Result (x, s')) \<in> f s \<Longrightarrow> (tr'', res) \<in> g x s'; tr = tr'' @ tr'\<rbrakk> \<Longrightarrow> P\<rbrakk>
+   \<Longrightarrow> P"
   by (auto simp: bind_def2)
 
-text \<open> Each monad satisfies at least the following three laws. \<close>
-
-text \<open> @{term return} is absorbed at the left of a @{term bind},
-  applying the return value directly: \<close>
+text \<open>Each monad satisfies at least the following three laws.\<close>
 
 declare map_option.identity[simp]
 
-lemma return_bind [simp]: "(return x >>= f) = f x"
-  by (auto simp add: return_def bind_def split_def split:if_splits)
+text \<open>@{term return} is absorbed at the left of a @{term bind}, applying the return value directly:\<close>
+lemma return_bind[simp]:
+  "(return x >>= f) = f x"
+  by (simp add: return_def bind_def)
 
-text \<open> @{term return} is absorbed on the right of a @{term bind} \<close>
-lemma bind_return [simp]: "(m >>= return) = m"
-  by (auto simp add: fun_eq_iff bind_def return_def
+text \<open>@{term return} is absorbed on the right of a @{term bind}\<close>
+lemma bind_return[simp]:
+  "(m >>= return) = m"
+  by (auto simp: fun_eq_iff bind_def return_def
            split: tmres.splits)
 
-text \<open> @{term bind} is associative \<close>
+text \<open>@{term bind} is associative\<close>
 lemma bind_assoc:
   fixes m :: "('a,'b) tmonad"
   fixes f :: "'b \<Rightarrow> ('a,'c) tmonad"
@@ -293,7 +238,7 @@ lemma bind_assoc:
   apply (simp add: image_image)
   done
 
-section \<open> Adding Exceptions \<close>
+section \<open>Adding Exceptions\<close>
 
 text \<open>
   The type @{typ "('s,'a) tmonad"} gives us nondeterminism and
@@ -309,95 +254,61 @@ text \<open>
   we provide new names for the @{term return} and @{term bind} functions
   in this monad. We call them @{text returnOk} (for normal return values)
   and @{text bindE} (for composition). We also define @{text throwError}
-  to return an exceptional value.
-\<close>
-definition
-  returnOk :: "'a \<Rightarrow> ('s, 'e + 'a) tmonad"
-where
+  to return an exceptional value.\<close>
+definition returnOk :: "'a \<Rightarrow> ('s, 'e + 'a) tmonad" where
   "returnOk \<equiv> return o Inr"
 
-definition
-  throwError :: "'e \<Rightarrow> ('s, 'e + 'a) tmonad"
-where
+definition throwError :: "'e \<Rightarrow> ('s, 'e + 'a) tmonad" where
   "throwError \<equiv> return o Inl"
 
 text \<open>
   Lifting a function over the exception type: if the input is an
-  exception, return that exception; otherwise continue execution.
-\<close>
-definition
-  lift :: "('a \<Rightarrow> ('s, 'e + 'b) tmonad) \<Rightarrow>
-           'e +'a \<Rightarrow> ('s, 'e + 'b) tmonad"
-where
-  "lift f v \<equiv> case v of Inl e \<Rightarrow> throwError e
-                      | Inr v' \<Rightarrow> f v'"
+  exception, return that exception; otherwise continue execution.\<close>
+definition lift :: "('a \<Rightarrow> ('s, 'e + 'b) tmonad) \<Rightarrow> 'e +'a \<Rightarrow> ('s, 'e + 'b) tmonad" where
+  "lift f v \<equiv> case v of Inl e \<Rightarrow> throwError e | Inr v' \<Rightarrow> f v'"
 
 text \<open>
   The definition of @{term bind} in the exception monad (new
   name @{text bindE}): the same as normal @{term bind}, but
   the right-hand side is skipped if the left-hand side
-  produced an exception.
-\<close>
-definition
-  bindE :: "('s, 'e + 'a) tmonad \<Rightarrow>
-            ('a \<Rightarrow> ('s, 'e + 'b) tmonad) \<Rightarrow>
-            ('s, 'e + 'b) tmonad"  (infixl ">>=E" 60)
-where
-  "bindE f g \<equiv> bind f (lift g)"
-
+  produced an exception.\<close>
+definition bindE ::
+  "('s, 'e + 'a) tmonad \<Rightarrow> ('a \<Rightarrow> ('s, 'e + 'b) tmonad) \<Rightarrow> ('s, 'e + 'b) tmonad"
+  (infixl ">>=E" 60) where
+  "f >>=E g \<equiv> f >>= lift g"
 
 text \<open>
   Lifting a normal nondeterministic monad into the
   exception monad is achieved by always returning its
-  result as normal result and never throwing an exception.
-\<close>
-definition
-  liftE :: "('s,'a) tmonad \<Rightarrow> ('s, 'e+'a) tmonad"
-where
+  result as normal result and never throwing an exception.\<close>
+definition liftE :: "('s,'a) tmonad \<Rightarrow> ('s, 'e+'a) tmonad" where
   "liftE f \<equiv> f >>= (\<lambda>r. return (Inr r))"
-
 
 text \<open>
   Since the underlying type and @{text return} function changed,
-  we need new definitions for when and unless:
-\<close>
-definition
-  whenE :: "bool \<Rightarrow> ('s, 'e + unit) tmonad \<Rightarrow>
-            ('s, 'e + unit) tmonad"
-where
+  we need new definitions for when and unless:\<close>
+definition whenE :: "bool \<Rightarrow> ('s, 'e + unit) tmonad \<Rightarrow> ('s, 'e + unit) tmonad" where
   "whenE P f \<equiv> if P then f else returnOk ()"
 
-definition
-  unlessE :: "bool \<Rightarrow> ('s, 'e + unit) tmonad \<Rightarrow>
-            ('s, 'e + unit) tmonad"
-where
+definition unlessE :: "bool \<Rightarrow> ('s, 'e + unit) tmonad \<Rightarrow> ('s, 'e + unit) tmonad" where
   "unlessE P f \<equiv> if P then returnOk () else f"
-
 
 text \<open>
   Throwing an exception when the parameter is @{term None}, otherwise
-  returning @{term "v"} for @{term "Some v"}.
-\<close>
-definition
-  throw_opt :: "'e \<Rightarrow> 'a option \<Rightarrow> ('s, 'e + 'a) tmonad"
-where
-  "throw_opt ex x \<equiv>
-    case x of None \<Rightarrow> throwError ex | Some v \<Rightarrow> returnOk v"
-
+  returning @{term "v"} for @{term "Some v"}.\<close>
+definition throw_opt :: "'e \<Rightarrow> 'a option \<Rightarrow> ('s, 'e + 'a) tmonad" where
+  "throw_opt ex x \<equiv> case x of None \<Rightarrow> throwError ex | Some v \<Rightarrow> returnOk v"
 
 text \<open>
   Failure in the exception monad is redefined in the same way
   as @{const whenE} and @{const unlessE}, with @{term returnOk}
-  instead of @{term return}.
-\<close>
-definition
-  assertE :: "bool \<Rightarrow> ('a, 'e + unit) tmonad"
-where
+  instead of @{term return}.\<close>
+definition assertE :: "bool \<Rightarrow> ('a, 'e + unit) tmonad" where
   "assertE P \<equiv> if P then returnOk () else fail"
 
 subsection "Monad Laws for the Exception Monad"
 
-text \<open> More direct definition of @{const liftE}: \<close>
+text \<open>More direct definition of @{const liftE}:\<close>
 lemma liftE_def2:
   "liftE f = (\<lambda>s. snd_upd (map_tmres_rv Inr) ` (f s))"
   apply (clarsimp simp: fun_eq_iff liftE_def return_def split_def bind_def image_def)
@@ -414,52 +325,51 @@ lemma liftE_def2:
   apply (clarsimp split: tmres.splits)
   done
 
-text \<open> Left @{const returnOk} absorbtion over @{term bindE}: \<close>
-lemma returnOk_bindE [simp]: "(returnOk x >>=E f) = f x"
-  apply (unfold bindE_def returnOk_def)
-  apply (clarsimp simp: lift_def)
-  done
+text \<open>Left @{const returnOk} absorbtion over @{term bindE}:\<close>
+lemma returnOk_bindE[simp]: "(returnOk x >>=E f) = f x"
+  unfolding bindE_def returnOk_def
+  by (clarsimp simp: lift_def)
 
-lemma lift_return [simp]:
+lemma lift_return[simp]:
   "lift (return \<circ> Inr) = return"
-  by (simp add: fun_eq_iff lift_def throwError_def split: sum.splits)
+  by (auto simp: lift_def throwError_def split: sum.splits)
 
-text \<open> Right @{const returnOk} absorbtion over @{term bindE}: \<close>
-lemma bindE_returnOk [simp]: "(m >>=E returnOk) = m"
+text \<open>Right @{const returnOk} absorbtion over @{term bindE}:\<close>
+lemma bindE_returnOk[simp]:
+  "(m >>=E returnOk) = m"
   by (simp add: bindE_def returnOk_def)
 
-text \<open> Associativity of @{const bindE}: \<close>
+text \<open>Associativity of @{const bindE}:\<close>
 lemma bindE_assoc:
   "(m >>=E f) >>=E g = m >>=E (\<lambda>x. f x >>=E g)"
-  apply (simp add: bindE_def bind_assoc)
-  apply (rule arg_cong [where f="\<lambda>x. m >>= x"])
-  apply (rule ext)
-  apply (case_tac x, simp_all add: lift_def throwError_def)
-  done
+  unfolding bindE_def
+  by (fastforce simp: bind_assoc lift_def throwError_def
+                split: sum.splits
+                intro: arg_cong[where f="\<lambda>x. m >>= x"])
 
-text \<open> @{const returnOk} could also be defined via @{const liftE}: \<close>
+text \<open>@{const returnOk} could also be defined via @{const liftE}:\<close>
 lemma returnOk_liftE:
   "returnOk x = liftE (return x)"
   by (simp add: liftE_def returnOk_def)
 
-text \<open> Execution after throwing an exception is skipped: \<close>
-lemma throwError_bindE [simp]:
+text \<open>Execution after throwing an exception is skipped:\<close>
+lemma throwError_bindE[simp]:
   "(throwError E >>=E f) = throwError E"
-  by (simp add: fun_eq_iff bindE_def bind_def throwError_def lift_def return_def split_def)
+  by (simp add: bindE_def bind_def throwError_def lift_def return_def)
 
 
 section "Syntax"
 
-text \<open> This section defines traditional Haskell-like do-syntax
-  for the state monad in Isabelle. \<close>
+text \<open>This section defines traditional Haskell-like do-syntax
+  for the state monad in Isabelle.\<close>
 
-subsection "Syntax for the Nondeterministic State Monad"
+subsection "Syntax for the Interference Trace Monad"
 
-text \<open> We use @{text K_bind} to syntactically indicate the
-  case where the return argument of the left side of a @{term bind}
-  is ignored \<close>
-definition
-  K_bind_def [iff]: "K_bind \<equiv> \<lambda>x y. x"
+text \<open>
+  We use @{text K_bind} to syntactically indicate the case where the return argument
+  of the left side of a @{term bind} is ignored\<close>
+definition K_bind :: "'a \<Rightarrow> 'b \<Rightarrow> 'a" where
+  K_bind_def[iff]: "K_bind \<equiv> \<lambda>x y. x"
 
 nonterminal
   dobinds and dobind and nobind
@@ -479,7 +389,7 @@ translations
   "_do (_nobind b) e"      == "b >>= (CONST K_bind e)"
   "do x <- a; e od"        == "a >>= (\<lambda>x. e)"
 
-text \<open> Syntax examples: \<close>
+text \<open>Syntax examples:\<close>
 lemma "do x \<leftarrow> return 1;
           return (2::nat);
           return x
@@ -495,58 +405,12 @@ lemma "do x \<leftarrow> return 1;
        od = return 1"
   by simp
 
-subsection "Interference command"
-
-text \<open>Interference commands must be inserted in between actions that can be interfered with commands
-running in other threads. \<close>
-
-definition
-  last_st_tr :: "(tmid * 's) list \<Rightarrow> 's \<Rightarrow> 's"
-where
-  "last_st_tr tr s0 = (hd (map snd tr @ [s0]))"
-
-definition
-  env_steps :: "('s,unit) tmonad"
-where
-  "env_steps \<equiv>
-  do
-    s \<leftarrow> get;
-    \<comment> \<open>Add unfiltered environment events to the trace\<close>
-    xs \<leftarrow> select UNIV;
-    tr \<leftarrow> return (map (Pair Env) xs);
-    put_trace tr;
-    \<comment> \<open>Pick the last event of the trace as the final state\<close>
-    put (last_st_tr tr s)
-  od"
-
-definition
-  commit_step :: "('s, unit) tmonad"
-where
-  "commit_step \<equiv>
-  do
-    s \<leftarrow> get;
-    put_trace [(Me,s)]
-  od"
-
-definition
-  interference :: "('s,unit) tmonad"
-where
-  "interference \<equiv>
-  do
-    commit_step;
-    env_steps
-  od"
-
 subsection "Syntax for the Exception Monad"
 
 text \<open>
-  Since the exception monad is a different type, we
-  need to syntactically distinguish it in the syntax.
-  We use @{text doE}/@{text odE} for this, but can re-use
-  most of the productions from @{text do}/@{text od}
-  above.
-\<close>
-
+  Since the exception monad is a different type, we need to distinguish it in the syntax
+  if we want to avoid ambiguous terms. We use @{text doE}/@{text odE} for this, but can
+  re-use most of the productions from @{text do}/@{text od} above. \<close>
 syntax
   "_doE" :: "[dobinds, 'a] => 'a"  ("(doE ((_);//(_))//odE)" 100)
 
@@ -555,7 +419,7 @@ translations
   "_doE (_nobind b) e"      == "b >>=E (CONST K_bind e)"
   "doE x <- a; e odE"       == "a >>=E (\<lambda>x. e)"
 
-text \<open> Syntax examples: \<close>
+text \<open>Syntax examples:\<close>
 lemma "doE x \<leftarrow> returnOk 1;
            returnOk (2::nat);
            returnOk x
@@ -572,107 +436,110 @@ lemma "doE x \<leftarrow> returnOk 1;
   by simp
 
 
+subsection "Interference command"
+
+text \<open>
+  Interference commands must be inserted in between actions that can be interfered with by
+  commands running in other threads.\<close>
+
+definition last_st_tr :: "(tmid * 's) list \<Rightarrow> 's \<Rightarrow> 's" where
+  "last_st_tr tr s0 \<equiv> hd (map snd tr @ [s0])"
+
+definition env_steps :: "('s,unit) tmonad" where
+  "env_steps \<equiv>
+  do
+    s \<leftarrow> get;
+    \<comment> \<open>Add unfiltered environment events to the trace\<close>
+    xs \<leftarrow> select UNIV;
+    tr \<leftarrow> return (map (Pair Env) xs);
+    put_trace tr;
+    \<comment> \<open>Pick the last event of the trace as the final state\<close>
+    put (last_st_tr tr s)
+  od"
+
+definition commit_step :: "('s,unit) tmonad" where
+  "commit_step \<equiv>
+  do
+    s \<leftarrow> get;
+    put_trace [(Me,s)]
+  od"
+
+definition interference :: "('s,unit) tmonad" where
+  "interference \<equiv>
+  do
+    commit_step;
+    env_steps
+  od"
+
 
 section "Library of additional Monadic Functions and Combinators"
 
-
-text \<open> Lifting a normal function into the monad type: \<close>
-definition
-  liftM :: "('a \<Rightarrow> 'b) \<Rightarrow> ('s,'a) tmonad \<Rightarrow> ('s, 'b) tmonad"
-where
+text \<open>Lifting a normal function into the monad type:\<close>
+definition liftM :: "('a \<Rightarrow> 'b) \<Rightarrow> ('s,'a) tmonad \<Rightarrow> ('s, 'b) tmonad" where
   "liftM f m \<equiv> do x \<leftarrow> m; return (f x) od"
 
-text \<open> The same for the exception monad: \<close>
-definition
-  liftME :: "('a \<Rightarrow> 'b) \<Rightarrow> ('s,'e+'a) tmonad \<Rightarrow> ('s,'e+'b) tmonad"
-where
+text \<open>The same for the exception monad:\<close>
+definition liftME :: "('a \<Rightarrow> 'b) \<Rightarrow> ('s,'e+'a) tmonad \<Rightarrow> ('s,'e+'b) tmonad" where
   "liftME f m \<equiv> doE x \<leftarrow> m; returnOk (f x) odE"
 
-text \<open> Run a sequence of monads from left to right, ignoring return values. \<close>
-definition
-  sequence_x :: "('s, 'a) tmonad list \<Rightarrow> ('s, unit) tmonad"
-where
+text \<open>Run a sequence of monads from left to right, ignoring return values.\<close>
+definition sequence_x :: "('s, 'a) tmonad list \<Rightarrow> ('s, unit) tmonad" where
   "sequence_x xs \<equiv> foldr (\<lambda>x y. x >>= (\<lambda>_. y)) xs (return ())"
 
 text \<open>
   Map a monadic function over a list by applying it to each element
-  of the list from left to right, ignoring return values.
-\<close>
-definition
-  mapM_x :: "('a \<Rightarrow> ('s,'b) tmonad) \<Rightarrow> 'a list \<Rightarrow> ('s, unit) tmonad"
-where
+  of the list from left to right, ignoring return values.\<close>
+definition mapM_x :: "('a \<Rightarrow> ('s,'b) tmonad) \<Rightarrow> 'a list \<Rightarrow> ('s, unit) tmonad" where
   "mapM_x f xs \<equiv> sequence_x (map f xs)"
 
 text \<open>
   Map a monadic function with two parameters over two lists,
   going through both lists simultaneously, left to right, ignoring
-  return values.
-\<close>
-definition
-  zipWithM_x :: "('a \<Rightarrow> 'b \<Rightarrow> ('s,'c) tmonad) \<Rightarrow>
-                 'a list \<Rightarrow> 'b list \<Rightarrow> ('s, unit) tmonad"
-where
+  return values.\<close>
+definition zipWithM_x ::
+  "('a \<Rightarrow> 'b \<Rightarrow> ('s,'c) tmonad) \<Rightarrow> 'a list \<Rightarrow> 'b list \<Rightarrow> ('s, unit) tmonad" where
   "zipWithM_x f xs ys \<equiv> sequence_x (zipWith f xs ys)"
 
-
-text \<open> The same three functions as above, but returning a list of
-return values instead of @{text unit} \<close>
-definition
-  sequence :: "('s, 'a) tmonad list \<Rightarrow> ('s, 'a list) tmonad"
-where
+text \<open>
+  The same three functions as above, but returning a list of
+  return values instead of @{text unit}\<close>
+definition sequence :: "('s, 'a) tmonad list \<Rightarrow> ('s, 'a list) tmonad" where
   "sequence xs \<equiv> let mcons = (\<lambda>p q. p >>= (\<lambda>x. q >>= (\<lambda>y. return (x#y))))
                  in foldr mcons xs (return [])"
 
-definition
-  mapM :: "('a \<Rightarrow> ('s,'b) tmonad) \<Rightarrow> 'a list \<Rightarrow> ('s, 'b list) tmonad"
-where
+definition mapM :: "('a \<Rightarrow> ('s,'b) tmonad) \<Rightarrow> 'a list \<Rightarrow> ('s, 'b list) tmonad" where
   "mapM f xs \<equiv> sequence (map f xs)"
 
-definition
-  zipWithM :: "('a \<Rightarrow> 'b \<Rightarrow> ('s,'c) tmonad) \<Rightarrow>
-                 'a list \<Rightarrow> 'b list \<Rightarrow> ('s, 'c list) tmonad"
-where
+definition zipWithM ::
+  "('a \<Rightarrow> 'b \<Rightarrow> ('s,'c) tmonad) \<Rightarrow> 'a list \<Rightarrow> 'b list \<Rightarrow> ('s, 'c list) tmonad" where
   "zipWithM f xs ys \<equiv> sequence (zipWith f xs ys)"
 
-definition
-  foldM :: "('b \<Rightarrow> 'a \<Rightarrow> ('s, 'a) tmonad) \<Rightarrow> 'b list \<Rightarrow> 'a \<Rightarrow> ('s, 'a) tmonad"
-where
+definition foldM :: "('b \<Rightarrow> 'a \<Rightarrow> ('s, 'a) tmonad) \<Rightarrow> 'b list \<Rightarrow> 'a \<Rightarrow> ('s, 'a) tmonad" where
   "foldM m xs a \<equiv> foldr (\<lambda>p q. q >>= m p) xs (return a) "
 
-definition
-  foldME ::"('b \<Rightarrow> 'a \<Rightarrow> ('s,('e + 'b)) tmonad) \<Rightarrow> 'b \<Rightarrow> 'a list \<Rightarrow> ('s, ('e + 'b)) tmonad"
-where "foldME m a xs \<equiv> foldr (\<lambda>p q. q >>=E swp m p) xs (returnOk a)"
+definition foldME ::
+  "('b \<Rightarrow> 'a \<Rightarrow> ('s,('e + 'b)) tmonad) \<Rightarrow> 'b \<Rightarrow> 'a list \<Rightarrow> ('s, ('e + 'b)) tmonad" where
+  "foldME m a xs \<equiv> foldr (\<lambda>p q. q >>=E swp m p) xs (returnOk a)"
 
-text \<open> The sequence and map functions above for the exception monad,
-with and without lists of return value \<close>
-definition
-  sequenceE_x :: "('s, 'e+'a) tmonad list \<Rightarrow> ('s, 'e+unit) tmonad"
-where
+text \<open>
+  The sequence and map functions above for the exception monad, with and without
+  lists of return value\<close>
+definition sequenceE_x :: "('s, 'e+'a) tmonad list \<Rightarrow> ('s, 'e+unit) tmonad" where
   "sequenceE_x xs \<equiv> foldr (\<lambda>x y. doE _ <- x; y odE) xs (returnOk ())"
 
-definition
-  mapME_x :: "('a \<Rightarrow> ('s,'e+'b) tmonad) \<Rightarrow> 'a list \<Rightarrow>
-              ('s,'e+unit) tmonad"
-where
+definition mapME_x :: "('a \<Rightarrow> ('s,'e+'b) tmonad) \<Rightarrow> 'a list \<Rightarrow> ('s,'e+unit) tmonad" where
   "mapME_x f xs \<equiv> sequenceE_x (map f xs)"
 
-definition
-  sequenceE :: "('s, 'e+'a) tmonad list \<Rightarrow> ('s, 'e+'a list) tmonad"
-where
+definition sequenceE :: "('s, 'e+'a) tmonad list \<Rightarrow> ('s, 'e+'a list) tmonad" where
   "sequenceE xs \<equiv> let mcons = (\<lambda>p q. p >>=E (\<lambda>x. q >>=E (\<lambda>y. returnOk (x#y))))
-                 in foldr mcons xs (returnOk [])"
+                   in foldr mcons xs (returnOk [])"
 
-definition
-  mapME :: "('a \<Rightarrow> ('s,'e+'b) tmonad) \<Rightarrow> 'a list \<Rightarrow>
-              ('s,'e+'b list) tmonad"
-where
+definition mapME :: "('a \<Rightarrow> ('s,'e+'b) tmonad) \<Rightarrow> 'a list \<Rightarrow> ('s,'e+'b list) tmonad" where
   "mapME f xs \<equiv> sequenceE (map f xs)"
 
 
-text \<open> Filtering a list using a monadic function as predicate: \<close>
-primrec
-  filterM :: "('a \<Rightarrow> ('s, bool) tmonad) \<Rightarrow> 'a list \<Rightarrow> ('s, 'a list) tmonad"
-where
+text \<open>Filtering a list using a monadic function as predicate:\<close>
+primrec filterM :: "('a \<Rightarrow> ('s, bool) tmonad) \<Rightarrow> 'a list \<Rightarrow> ('s, 'a list) tmonad" where
   "filterM P []       = return []"
 | "filterM P (x # xs) = do
      b  <- P x;
@@ -680,13 +547,10 @@ where
      return (if b then (x # ys) else ys)
    od"
 
-text \<open> @{text select_state} takes a relationship between
-  states, and outputs nondeterministically a state
-  related to the input state. \<close>
-
-definition
-  state_select :: "('s \<times> 's) set \<Rightarrow> ('s, unit) tmonad"
-where
+text \<open>
+  @{text select_state} takes a relationship between states, and outputs
+  nondeterministically a state related to the input state.\<close>
+definition state_select :: "('s \<times> 's) set \<Rightarrow> ('s, unit) tmonad" where
   "state_select r \<equiv> (do
     s \<leftarrow> get;
     S \<leftarrow> return {s'. (s, s') \<in> r};
@@ -694,17 +558,15 @@ where
     s' \<leftarrow> select S;
     put s'
   od)"
+
+
 section "Catching and Handling Exceptions"
 
 text \<open>
   Turning an exception monad into a normal state monad
-  by catching and handling any potential exceptions:
-\<close>
-definition
-  catch :: "('s, 'e + 'a) tmonad \<Rightarrow>
-            ('e \<Rightarrow> ('s, 'a) tmonad) \<Rightarrow>
-            ('s, 'a) tmonad" (infix "<catch>" 10)
-where
+  by catching and handling any potential exceptions:\<close>
+definition catch ::
+  "('s, 'e + 'a) tmonad \<Rightarrow> ('e \<Rightarrow> ('s, 'a) tmonad) \<Rightarrow> ('s, 'a) tmonad" (infix "<catch>" 10) where
   "f <catch> handler \<equiv>
      do x \<leftarrow> f;
         case x of
@@ -715,13 +577,10 @@ where
 text \<open>
   Handling exceptions, but staying in the exception monad.
   The handler may throw a type of exceptions different from
-  the left side.
-\<close>
-definition
-  handleE' :: "('s, 'e1 + 'a) tmonad \<Rightarrow>
-               ('e1 \<Rightarrow> ('s, 'e2 + 'a) tmonad) \<Rightarrow>
-               ('s, 'e2 + 'a) tmonad" (infix "<handle2>" 10)
-where
+  the left side.\<close>
+definition handleE' ::
+  "('s, 'e1 + 'a) tmonad \<Rightarrow> ('e1 \<Rightarrow> ('s, 'e2 + 'a) tmonad) \<Rightarrow> ('s, 'e2 + 'a) tmonad"
+  (infix "<handle2>" 10) where
   "f <handle2> handler \<equiv>
    do
       v \<leftarrow> f;
@@ -733,27 +592,19 @@ where
 text \<open>
   A type restriction of the above that is used more commonly in
   practice: the exception handle (potentially) throws exception
-  of the same type as the left-hand side.
-\<close>
-definition
-  handleE :: "('s, 'x + 'a) tmonad \<Rightarrow>
-              ('x \<Rightarrow> ('s, 'x + 'a) tmonad) \<Rightarrow>
-              ('s, 'x + 'a) tmonad" (infix "<handle>" 10)
-where
+  of the same type as the left-hand side.\<close>
+definition handleE ::
+  "('s, 'x + 'a) tmonad \<Rightarrow> ('x \<Rightarrow> ('s, 'x + 'a) tmonad) \<Rightarrow> ('s, 'x + 'a) tmonad"
+  (infix "<handle>" 10) where
   "handleE \<equiv> handleE'"
-
 
 text \<open>
   Handling exceptions, and additionally providing a continuation
-  if the left-hand side throws no exception:
-\<close>
-definition
-  handle_elseE :: "('s, 'e + 'a) tmonad \<Rightarrow>
-                   ('e \<Rightarrow> ('s, 'ee + 'b) tmonad) \<Rightarrow>
-                   ('a \<Rightarrow> ('s, 'ee + 'b) tmonad) \<Rightarrow>
-                   ('s, 'ee + 'b) tmonad"
-  ("_ <handle> _ <else> _" 10)
-where
+  if the left-hand side throws no exception:\<close>
+definition handle_elseE ::
+  "('s, 'e + 'a) tmonad \<Rightarrow> ('e \<Rightarrow> ('s, 'ee + 'b) tmonad) \<Rightarrow> ('a \<Rightarrow> ('s, 'ee + 'b) tmonad) \<Rightarrow>
+   ('s, 'ee + 'b) tmonad"
+  ("_ <handle> _ <else> _" 10) where
   "f <handle> handler <else> continue \<equiv>
    do v \<leftarrow> f;
    case v of Inl e  \<Rightarrow> handler e
@@ -765,57 +616,53 @@ subsection "Loops"
 text \<open>
   Loops are handled using the following inductive predicate;
   non-termination is represented using the failure flag of the
-  monad.
-\<close>
-inductive_set
-  whileLoop_results :: "('r \<Rightarrow> 's \<Rightarrow> bool) \<Rightarrow> ('r \<Rightarrow> ('s, 'r) tmonad) \<Rightarrow> (('r \<times> 's) \<times> ((tmid \<times> 's) list \<times> ('s, 'r) tmres)) set"
-  for C B
-where
+  monad.\<close>
+
+inductive_set whileLoop_results ::
+  "('r \<Rightarrow> 's \<Rightarrow> bool) \<Rightarrow> ('r \<Rightarrow> ('s, 'r) tmonad) \<Rightarrow> (('r \<times> 's) \<times> ((tmid \<times> 's) list \<times> ('s, 'r) tmres)) set"
+  for C B where
     "\<lbrakk> \<not> C r s \<rbrakk> \<Longrightarrow> ((r, s), ([], Result (r, s))) \<in> whileLoop_results C B"
   | "\<lbrakk> C r s; (ts, Failed) \<in> B r s \<rbrakk> \<Longrightarrow> ((r, s), (ts, Failed)) \<in> whileLoop_results C B"
   | "\<lbrakk> C r s; (ts, Incomplete) \<in> B r s \<rbrakk> \<Longrightarrow> ((r, s), (ts, Incomplete)) \<in> whileLoop_results C B"
   | "\<lbrakk> C r s; (ts, Result (r', s')) \<in> B r s; ((r', s'), (ts',z)) \<in> whileLoop_results C B  \<rbrakk>
        \<Longrightarrow> ((r, s), (ts'@ts,z)) \<in> whileLoop_results C B"
 
+\<comment> \<open>FIXME: there are fewer lemmas here than in NonDetMonad and I don't understand this well enough
+  to know whether this is correct or not.\<close>
 inductive_cases whileLoop_results_cases_result_end: "((x,y), ([],Result r)) \<in> whileLoop_results C B"
 inductive_cases whileLoop_results_cases_fail: "((x,y), (ts, Failed)) \<in> whileLoop_results C B"
 inductive_cases whileLoop_results_cases_incomplete: "((x,y), (ts, Incomplete)) \<in> whileLoop_results C B"
 
 inductive_simps whileLoop_results_simps_valid: "((x,y), ([], Result z)) \<in> whileLoop_results C B"
 
-inductive
-  whileLoop_terminates :: "('r \<Rightarrow> 's \<Rightarrow> bool) \<Rightarrow> ('r \<Rightarrow> ('s, 'r) tmonad) \<Rightarrow> 'r \<Rightarrow> 's \<Rightarrow> bool"
-  for C B
-where
+inductive whileLoop_terminates ::
+  "('r \<Rightarrow> 's \<Rightarrow> bool) \<Rightarrow> ('r \<Rightarrow> ('s, 'r) tmonad) \<Rightarrow> 'r \<Rightarrow> 's \<Rightarrow> bool"
+  for C B where
     "\<not> C r s \<Longrightarrow> whileLoop_terminates C B r s"
   | "\<lbrakk> C r s; \<forall>(r', s') \<in> Result -` snd ` (B r s). whileLoop_terminates C B r' s' \<rbrakk>
         \<Longrightarrow> whileLoop_terminates C B r s"
 
-
 inductive_cases whileLoop_terminates_cases: "whileLoop_terminates C B r s"
 inductive_simps whileLoop_terminates_simps: "whileLoop_terminates C B r s"
 
-definition
-  whileLoop :: "('r \<Rightarrow> 's \<Rightarrow> bool) \<Rightarrow> ('r \<Rightarrow> ('s, 'r) tmonad) \<Rightarrow> 'r \<Rightarrow> ('s, 'r) tmonad"
-where
+definition whileLoop ::
+  "('r \<Rightarrow> 's \<Rightarrow> bool) \<Rightarrow> ('r \<Rightarrow> ('s, 'r) tmonad) \<Rightarrow> 'r \<Rightarrow> ('s, 'r) tmonad" where
   "whileLoop C B \<equiv> (\<lambda>r s. {(ts, res). ((r,s), ts,res) \<in> whileLoop_results C B})"
 
 notation (output)
   whileLoop  ("(whileLoop (_)//  (_))" [1000, 1000] 1000)
 
-definition
-  whileLoopT :: "('r \<Rightarrow> 's \<Rightarrow> bool) \<Rightarrow> ('r \<Rightarrow> ('s, 'r) tmonad) \<Rightarrow> 'r \<Rightarrow> ('s, 'r) tmonad"
-where
+\<comment> \<open>FIXME: why does this differ to Nondet_Monad?\<close>
+definition whileLoopT ::
+  "('r \<Rightarrow> 's \<Rightarrow> bool) \<Rightarrow> ('r \<Rightarrow> ('s, 'r) tmonad) \<Rightarrow> 'r \<Rightarrow> ('s, 'r) tmonad" where
   "whileLoopT C B \<equiv> (\<lambda>r s. {(ts, res). ((r,s), ts,res) \<in> whileLoop_results C B
                                          \<and> whileLoop_terminates C B r s})"
 
 notation (output)
   whileLoopT  ("(whileLoopT (_)//  (_))" [1000, 1000] 1000)
 
-definition
-  whileLoopE :: "('r \<Rightarrow> 's \<Rightarrow> bool) \<Rightarrow> ('r \<Rightarrow> ('s, 'e + 'r) tmonad)
-      \<Rightarrow> 'r \<Rightarrow> ('s, ('e + 'r)) tmonad"
-where
+definition whileLoopE ::
+  "('r \<Rightarrow> 's \<Rightarrow> bool) \<Rightarrow> ('r \<Rightarrow> ('s, 'e + 'r) tmonad) \<Rightarrow> 'r \<Rightarrow> ('s, ('e + 'r)) tmonad" where
   "whileLoopE C body \<equiv>
       \<lambda>r. whileLoop (\<lambda>r s. (case r of Inr v \<Rightarrow> C v s | _ \<Rightarrow> False)) (lift body) (Inr r)"
 
@@ -824,13 +671,9 @@ notation (output)
 
 subsection "Await command"
 
-text \<open> @{term "Await c f"} blocks the execution until the @{term "c"} is true,
-      and atomically executes @{term "f"}.
-\<close>
-
-definition
-  Await :: "('s \<Rightarrow> bool) \<Rightarrow> ('s,unit) tmonad"
-where
+text \<open>@{term "Await c f"} blocks the execution until @{term "c"} is true,
+      and then atomically executes @{term "f"}.\<close>
+definition Await :: "('s \<Rightarrow> bool) \<Rightarrow> ('s,unit) tmonad" where
   "Await c \<equiv>
   do
     s \<leftarrow> get;
@@ -843,19 +686,21 @@ where
     put (last_st_tr tr s)
   od"
 
+
 section "Hoare Logic"
 
 subsection "Validity"
 
-text \<open> This section defines a Hoare logic for partial correctness for
-  the nondeterministic state monad as well as the exception monad.
+text \<open>
+  This section defines a Hoare logic for partial correctness for
+  the interference trace monad as well as the exception monad.
   The logic talks only about the behaviour part of the monad and ignores
   the failure flag.
 
   The logic is defined semantically. Rules work directly on the
   validity predicate.
 
-  In the nondeterministic state monad, validity is a triple of precondition,
+  In the interference trace monad, validity is a triple of precondition,
   monad, and postcondition. The precondition is a function from state to
   bool (a state predicate), the postcondition is a function from return value
   to state to bool. A triple is valid if for all states that satisfy the
@@ -864,52 +709,40 @@ text \<open> This section defines a Hoare logic for partial correctness for
   the empty set, the triple is trivially valid. This means @{term "assert P"}
   does not require us to prove that @{term P} holds, but rather allows us
   to assume @{term P}! Proving non-failure is done via separate predicate and
-  calculus (see below).
-\<close>
+  calculus (see below).\<close>
 
-
-definition
-  valid :: "('s \<Rightarrow> bool) \<Rightarrow> ('s,'a) tmonad \<Rightarrow> ('a \<Rightarrow> 's \<Rightarrow> bool) \<Rightarrow> bool"
-  ("\<lbrace>_\<rbrace>/ _ /\<lbrace>_\<rbrace>")
-where
+definition valid :: "('s \<Rightarrow> bool) \<Rightarrow> ('s,'a) tmonad \<Rightarrow> ('a \<Rightarrow> 's \<Rightarrow> bool) \<Rightarrow> bool"
+  ("\<lbrace>_\<rbrace>/ _ /\<lbrace>_\<rbrace>") where
   "\<lbrace>P\<rbrace> f \<lbrace>Q\<rbrace> \<equiv> \<forall>s. P s \<longrightarrow> (\<forall>(r,s') \<in> mres (f s). Q r s')"
 
 text \<open>
   We often reason about invariant predicates. The following provides shorthand syntax
-  that avoids repeating potentially long predicates.
-\<close>
-abbreviation (input)
-  invariant :: "('s,'a) tmonad \<Rightarrow> ('s \<Rightarrow> bool) \<Rightarrow> bool" ("_ \<lbrace>_\<rbrace>" [59,0] 60)
-where
+  that avoids repeating potentially long predicates.\<close>
+abbreviation (input) invariant ::
+  "('s,'a) tmonad \<Rightarrow> ('s \<Rightarrow> bool) \<Rightarrow> bool" ("_ \<lbrace>_\<rbrace>" [59,0] 60) where
   "invariant f P \<equiv> \<lbrace>P\<rbrace> f \<lbrace>\<lambda>_. P\<rbrace>"
-
-text \<open>rg_pred type: Rely-Guaranty predicates (state before => state after => bool)\<close>
-type_synonym 's rg_pred = "'s \<Rightarrow> 's \<Rightarrow> bool"
-
 
 text \<open>
   Validity for the exception monad is similar and build on the standard
   validity above. Instead of one postcondition, we have two: one for
-  normal and one for exceptional results.
-\<close>
-definition
-  validE :: "('s \<Rightarrow> bool) \<Rightarrow> ('s, 'a + 'b) tmonad \<Rightarrow>
-             ('b \<Rightarrow> 's \<Rightarrow> bool) \<Rightarrow>
-             ('a \<Rightarrow> 's \<Rightarrow> bool) \<Rightarrow> bool"
-("\<lbrace>_\<rbrace>/ _ /(\<lbrace>_\<rbrace>,/ \<lbrace>_\<rbrace>)" )
-where
+  normal and one for exceptional results.\<close>
+definition validE ::
+  "('s \<Rightarrow> bool) \<Rightarrow> ('s, 'a + 'b) tmonad \<Rightarrow> ('b \<Rightarrow> 's \<Rightarrow> bool) \<Rightarrow> ('a \<Rightarrow> 's \<Rightarrow> bool) \<Rightarrow> bool"
+  ("\<lbrace>_\<rbrace>/ _ /(\<lbrace>_\<rbrace>,/ \<lbrace>_\<rbrace>)" ) where
   "\<lbrace>P\<rbrace> f \<lbrace>Q\<rbrace>,\<lbrace>E\<rbrace> \<equiv> \<lbrace>P\<rbrace> f \<lbrace> \<lambda>v s. case v of Inr r \<Rightarrow> Q r s | Inl e \<Rightarrow> E e s \<rbrace>"
+
+lemma validE_def2:
+  "\<lbrace>P\<rbrace> f \<lbrace>Q\<rbrace>,\<lbrace>E\<rbrace> \<equiv> \<forall>s. P s \<longrightarrow> (\<forall>(r,s') \<in> mres (f s). case r of Inr b \<Rightarrow> Q b s' | Inl a \<Rightarrow> E a s')"
+  by (unfold valid_def validE_def)
 (*
-text \<open> Validity for exception monad with interferences. Not as easy to phrase
- as we need to  \<close>
-definition
-  validIE :: "('s, 'a + 'b) tmonad \<Rightarrow>
+text \<open>Validity for exception monad with interferences. Not as easy to phrase
+ as we need to \<close>
+definition validIE :: "('s, 'a + 'b) tmonad \<Rightarrow>
              's rg_pred \<Rightarrow>
              's rg_pred \<Rightarrow> 's rg_pred \<Rightarrow>
              ('b \<Rightarrow> 's rg_pred) \<Rightarrow>
              ('a \<Rightarrow> 's rg_pred) \<Rightarrow> bool"
- ("_ //PRE _//RELY _//GUAR _//POST _//EXC _" [59,0,0,0,0,0] 60)
-where
+ ("_ //PRE _//RELY _//GUAR _//POST _//EXC _" [59,0,0,0,0,0] 60) where
   "validIE f P R G Q E \<equiv> f SAT [P,R,G,\<lambda>v. case v of Inr r \<Rightarrow> Q r | Inl e \<Rightarrow> E e]"
 
 abbreviation (input)
@@ -923,81 +756,66 @@ abbreviation (input)
   "validIEsat f P R G Q E \<equiv> validIE f P R G Q E"
  *)
 text \<open>
-  The following two instantiations are convenient to separate reasoning
-  for exceptional and normal case.
-\<close>
-definition
-  validE_R :: "('s \<Rightarrow> bool) \<Rightarrow> ('s, 'e + 'a) tmonad \<Rightarrow>
-               ('a \<Rightarrow> 's \<Rightarrow> bool) \<Rightarrow> bool"
-   ("\<lbrace>_\<rbrace>/ _ /\<lbrace>_\<rbrace>, -")
-where
+  The following two instantiations are convenient to separate reasoning for exceptional and
+  normal case.\<close>
+(* Narrator: they are in fact not convenient, and are now considered a mistake that should have
+             been an abbreviation instead. *)
+definition validE_R :: (* FIXME lib: this should be an abbreviation *)
+  "('s \<Rightarrow> bool) \<Rightarrow> ('s, 'e + 'a) tmonad \<Rightarrow> ('a \<Rightarrow> 's \<Rightarrow> bool) \<Rightarrow> bool" ("\<lbrace>_\<rbrace>/ _ /\<lbrace>_\<rbrace>, -") where
   "\<lbrace>P\<rbrace> f \<lbrace>Q\<rbrace>,- \<equiv> validE P f Q (\<lambda>x y. True)"
 
-definition
-  validE_E :: "('s \<Rightarrow> bool) \<Rightarrow>  ('s, 'e + 'a) tmonad \<Rightarrow>
-               ('e \<Rightarrow> 's \<Rightarrow> bool) \<Rightarrow> bool"
-   ("\<lbrace>_\<rbrace>/ _ /-, \<lbrace>_\<rbrace>")
-where
+definition validE_E :: (* FIXME lib: this should be an abbreviation *)
+  "('s \<Rightarrow> bool) \<Rightarrow>  ('s, 'e + 'a) tmonad \<Rightarrow> ('e \<Rightarrow> 's \<Rightarrow> bool) \<Rightarrow> bool" ("\<lbrace>_\<rbrace>/ _ /-, \<lbrace>_\<rbrace>") where
   "\<lbrace>P\<rbrace> f -,\<lbrace>Q\<rbrace> \<equiv> validE P f (\<lambda>x y. True) Q"
 
 
-text \<open> Abbreviations for trivial postconditions (taking three arguments): \<close>
+text \<open>rg_pred type: Rely-Guaranty predicates (state before => state after => bool)\<close>
+type_synonym 's rg_pred = "'s \<Rightarrow> 's \<Rightarrow> bool"
+
+text \<open>Abbreviations for trivial postconditions (taking three arguments):\<close>
 abbreviation(input)
-  toptoptop :: "'a \<Rightarrow> 'b \<Rightarrow> 'b \<Rightarrow> bool" ("\<top>\<top>\<top>")
-where
+  toptoptop :: "'a \<Rightarrow> 'b \<Rightarrow> 'b \<Rightarrow> bool" ("\<top>\<top>\<top>") where
   "\<top>\<top>\<top> \<equiv> \<lambda>_ _ _. True"
 
 abbreviation(input)
-  botbotbot :: "'a \<Rightarrow> 'b \<Rightarrow> 'b \<Rightarrow> bool" ("\<bottom>\<bottom>\<bottom>")
-where
+  botbotbot :: "'a \<Rightarrow> 'b \<Rightarrow> 'b \<Rightarrow> bool" ("\<bottom>\<bottom>\<bottom>") where
   "\<bottom>\<bottom>\<bottom> \<equiv> \<lambda>_ _ _. False"
 
 
 subsection "Determinism"
 
-text \<open> A monad of type @{text tmonad} is deterministic iff it
-returns an empty trace, exactly one state and result and does not fail \<close>
-definition
-  det :: "('a,'s) tmonad \<Rightarrow> bool"
-where
+text \<open>
+  A monad of type @{text tmonad} is deterministic iff it
+  returns an empty trace, exactly one state and result and does not fail\<close>
+definition det :: "('a,'s) tmonad \<Rightarrow> bool" where
   "det f \<equiv> \<forall>s. \<exists>r. f s = {([], Result r)}"
 
-text \<open> A deterministic @{text tmonad} can be turned
-  into a normal state monad: \<close>
-definition
-  the_run_state :: "('s,'a) tmonad \<Rightarrow> 's \<Rightarrow> 'a \<times> 's"
-where
+text \<open>A deterministic @{text tmonad} can be turned into a normal state monad:\<close>
+definition the_run_state :: "('s,'a) tmonad \<Rightarrow> 's \<Rightarrow> 'a \<times> 's" where
   "the_run_state M \<equiv> \<lambda>s. THE s'. mres (M s) = {s'}"
 
 
 subsection "Non-Failure"
 
 text \<open>
-  We can formulate non-failure separately from validity.
+  With the failure flag, we can formulate non-failure separately from validity.
+  A monad @{text m} does not fail under precondition @{text P}, if for no start
+  state that satisfies the precondition it sets the failure flag.
 \<close>
-definition
-  no_fail :: "('s \<Rightarrow> bool) \<Rightarrow> ('s,'a) tmonad \<Rightarrow> bool"
-where
+definition no_fail :: "('s \<Rightarrow> bool) \<Rightarrow> ('s,'a) tmonad \<Rightarrow> bool" where
   "no_fail P m \<equiv> \<forall>s. P s \<longrightarrow> Failed \<notin> snd ` (m s)"
 
 text \<open>
-  It is often desired to prove non-failure and a Hoare triple
-  simultaneously, as the reasoning is often similar. The following
-  definitions allow such reasoning to take place.
-\<close>
+  It is often desired to prove non-failure and a Hoare triple simultaneously, as the reasoning
+  is often similar. The following definitions allow such reasoning to take place.\<close>
 
-definition
-  validNF ::"('s \<Rightarrow> bool) \<Rightarrow> ('s,'a) tmonad \<Rightarrow> ('a \<Rightarrow> 's \<Rightarrow> bool) \<Rightarrow> bool"
-      ("\<lbrace>_\<rbrace>/ _ /\<lbrace>_\<rbrace>!")
-where
+definition validNF ::
+  "('s \<Rightarrow> bool) \<Rightarrow> ('s,'a) tmonad \<Rightarrow> ('a \<Rightarrow> 's \<Rightarrow> bool) \<Rightarrow> bool" ("\<lbrace>_\<rbrace>/ _ /\<lbrace>_\<rbrace>!") where
   "validNF P f Q \<equiv> valid P f Q \<and> no_fail P f"
 
-definition
-  validE_NF :: "('s \<Rightarrow> bool) \<Rightarrow> ('s, 'a + 'b) tmonad \<Rightarrow>
-             ('b \<Rightarrow> 's \<Rightarrow> bool) \<Rightarrow>
-             ('a \<Rightarrow> 's \<Rightarrow> bool) \<Rightarrow> bool"
-  ("\<lbrace>_\<rbrace>/ _ /(\<lbrace>_\<rbrace>,/ \<lbrace>_\<rbrace>!)")
-where
+definition validE_NF ::
+  "('s \<Rightarrow> bool) \<Rightarrow> ('s, 'a + 'b) tmonad \<Rightarrow> ('b \<Rightarrow> 's \<Rightarrow> bool) \<Rightarrow> ('a \<Rightarrow> 's \<Rightarrow> bool) \<Rightarrow> bool"
+  ("\<lbrace>_\<rbrace>/ _ /(\<lbrace>_\<rbrace>,/ \<lbrace>_\<rbrace>!)") where
   "validE_NF P f Q E \<equiv> validE P f Q E \<and> no_fail P f"
 
 lemma validE_NF_alt_def:
@@ -1007,39 +825,31 @@ lemma validE_NF_alt_def:
 (* text \<open>
   Usually, well-formed monads constructed from the primitives
   above will have the following property: if they return an
-  empty set of results, they will have the failure flag set.
-\<close>
-definition
-  empty_fail :: "('s,'a) tmonad \<Rightarrow> bool"
-where
+  empty set of results, they will have the failure flag set.\<close>
+definition empty_fail :: "('s,'a) tmonad \<Rightarrow> bool" where
   "empty_fail m \<equiv> \<forall>s. fst (m s) = {} \<longrightarrow> snd (m s)"
 
 text \<open>
   Useful in forcing otherwise unknown executions to have
-  the @{const empty_fail} property.
-\<close>
-definition
-  mk_ef :: "'a set \<times> bool \<Rightarrow> 'a set \<times> bool"
-where
+  the @{const empty_fail} property.\<close>
+definition mk_ef :: "'a set \<times> bool \<Rightarrow> 'a set \<times> bool" where
   "mk_ef S \<equiv> (fst S, fst S = {} \<or> snd S)"
  *)
 section "Basic exception reasoning"
 
 text \<open>
-  The following predicates @{text no_throw} and @{text no_return} allow
-  reasoning that functions in the exception monad either do
-  no throw an exception or never return normally.
-\<close>
+  The predicates @{text no_throw} and @{text no_return} allow us to reason about functions in
+  the exception monad that never throw an exception or never return normally.\<close>
 
-definition "no_throw P A \<equiv> \<lbrace> P \<rbrace> A \<lbrace> \<lambda>_ _. True \<rbrace>,\<lbrace> \<lambda>_ _. False \<rbrace>"
+definition no_throw :: "('s \<Rightarrow> bool) \<Rightarrow> ('s, 'e + 'a) tmonad \<Rightarrow> bool" where
+  "no_throw P A \<equiv> \<lbrace> P \<rbrace> A \<lbrace> \<lambda>_ _. True \<rbrace>,\<lbrace> \<lambda>_ _. False \<rbrace>"
 
-definition "no_return P A \<equiv> \<lbrace> P \<rbrace> A \<lbrace>\<lambda>_ _. False\<rbrace>,\<lbrace>\<lambda>_ _. True \<rbrace>"
+definition no_return :: "('a \<Rightarrow> bool) \<Rightarrow> ('a, 'b + 'c) tmonad \<Rightarrow> bool" where
+  "no_return P A \<equiv> \<lbrace> P \<rbrace> A \<lbrace>\<lambda>_ _. False\<rbrace>,\<lbrace>\<lambda>_ _. True \<rbrace>"
 
 section "Trace monad Parallel"
 
-definition
-  parallel :: "('s,'a) tmonad \<Rightarrow> ('s,'a) tmonad \<Rightarrow> ('s,'a) tmonad"
-where
+definition parallel :: "('s,'a) tmonad \<Rightarrow> ('s,'a) tmonad \<Rightarrow> ('s,'a) tmonad" where
   "parallel f g = (\<lambda>s. {(xs, rv). \<exists>f_steps. length f_steps = length xs
     \<and> (map (\<lambda>(f_step, (id, s)). (if f_step then id else Env, s)) (zip f_steps xs), rv) \<in> f s
     \<and> (map (\<lambda>(f_step, (id, s)). (if f_step then Env else id, s)) (zip f_steps xs), rv) \<in> g s})"
@@ -1072,8 +882,7 @@ lemma parallel_def3:
   by (simp add: parallel_def2, rule ext, auto simp: image_def)
 
 primrec
-  trace_steps :: "(tmid \<times> 's) list \<Rightarrow> 's \<Rightarrow> (tmid \<times> 's \<times> 's) set"
-where
+  trace_steps :: "(tmid \<times> 's) list \<Rightarrow> 's \<Rightarrow> (tmid \<times> 's \<times> 's) set" where
   "trace_steps (elem # trace) s0 = {(fst elem, s0, snd elem)} \<union> trace_steps trace (snd elem)"
 | "trace_steps [] s0 = {}"
 
@@ -1091,14 +900,10 @@ next
     done
 qed
 
-definition
-  rely_cond :: "'s rg_pred \<Rightarrow> 's \<Rightarrow> (tmid \<times> 's) list \<Rightarrow> bool"
-where
+definition rely_cond :: "'s rg_pred \<Rightarrow> 's \<Rightarrow> (tmid \<times> 's) list \<Rightarrow> bool" where
   "rely_cond R s0s tr = (\<forall>(ident, s0, s) \<in> trace_steps (rev tr) s0s. ident = Env \<longrightarrow> R s0 s)"
 
-definition
-  guar_cond :: "'s rg_pred \<Rightarrow> 's \<Rightarrow> (tmid \<times> 's) list \<Rightarrow> bool"
-where
+definition guar_cond :: "'s rg_pred \<Rightarrow> 's \<Rightarrow> (tmid \<times> 's) list \<Rightarrow> bool" where
   "guar_cond G s0s tr = (\<forall>(ident, s0, s) \<in> trace_steps (rev tr) s0s. ident = Me \<longrightarrow> G s0 s)"
 
 lemma rg_empty_conds[simp]:
@@ -1106,21 +911,15 @@ lemma rg_empty_conds[simp]:
   "guar_cond G s0s []"
   by (simp_all add: rely_cond_def guar_cond_def)
 
-definition
-  rely :: "('s, 'a) tmonad \<Rightarrow> 's rg_pred \<Rightarrow> 's \<Rightarrow> ('s, 'a) tmonad"
-where
+definition rely :: "('s, 'a) tmonad \<Rightarrow> 's rg_pred \<Rightarrow> 's \<Rightarrow> ('s, 'a) tmonad" where
   "rely f R s0s \<equiv> (\<lambda>s. f s \<inter> ({tr. rely_cond R s0s tr} \<times> UNIV))"
 
-definition
-  prefix_closed :: "('s, 'a) tmonad \<Rightarrow> bool"
-where
+definition prefix_closed :: "('s, 'a) tmonad \<Rightarrow> bool" where
   "prefix_closed f = (\<forall>s. \<forall>x xs. (x # xs) \<in> fst ` f s \<longrightarrow> (xs, Incomplete) \<in> f s)"
 
-definition
-  validI :: "('s \<Rightarrow> 's \<Rightarrow> bool) \<Rightarrow> 's rg_pred \<Rightarrow> ('s,'a) tmonad
-    \<Rightarrow> 's rg_pred \<Rightarrow> ('a \<Rightarrow> 's \<Rightarrow> 's \<Rightarrow> bool) \<Rightarrow> bool"
-  ("(\<lbrace>_\<rbrace>,/ \<lbrace>_\<rbrace>)/ _ /(\<lbrace>_\<rbrace>,/ \<lbrace>_\<rbrace>)")
-where
+definition validI ::
+  "('s \<Rightarrow> 's \<Rightarrow> bool) \<Rightarrow> 's rg_pred \<Rightarrow> ('s,'a) tmonad \<Rightarrow> 's rg_pred \<Rightarrow> ('a \<Rightarrow> 's \<Rightarrow> 's \<Rightarrow> bool) \<Rightarrow> bool"
+  ("(\<lbrace>_\<rbrace>,/ \<lbrace>_\<rbrace>)/ _ /(\<lbrace>_\<rbrace>,/ \<lbrace>_\<rbrace>)") where
   "\<lbrace>P\<rbrace>,\<lbrace>R\<rbrace> f \<lbrace>G\<rbrace>,\<lbrace>Q\<rbrace> \<equiv> prefix_closed f \<and> (\<forall>s0 s. P s0 s
     \<longrightarrow> (\<forall>tr res. (tr, res) \<in> (rely f R s0 s) \<longrightarrow> guar_cond G s0 tr
         \<and> (\<forall>rv s'. res = Result (rv, s') \<longrightarrow> Q rv (last_st_tr tr s0) s')))"
@@ -1129,13 +928,14 @@ lemma in_rely:
   "\<lbrakk> (tr, res) \<in> f s; rely_cond R s0s tr \<rbrakk> \<Longrightarrow> (tr, res) \<in> rely f R s0s s"
   by (simp add: rely_def)
 
-lemmas validI_D = validI_def[THEN meta_eq_to_obj_eq, THEN iffD1,
-    THEN conjunct2, rule_format, OF _ _ in_rely]
+lemmas validI_D =
+  validI_def[THEN meta_eq_to_obj_eq, THEN iffD1, THEN conjunct2, rule_format, OF _ _ in_rely]
 lemmas validI_GD = validI_D[THEN conjunct1]
 lemmas validI_rvD = validI_D[THEN conjunct2, rule_format, rotated -1, OF refl]
 lemmas validI_prefix_closed = validI_def[THEN meta_eq_to_obj_eq, THEN iffD1, THEN conjunct1]
-lemmas validI_prefix_closed_T = validI_prefix_closed[where P="\<lambda>_ _. False" and R="\<lambda>_ _. False"
-    and G="\<lambda>_ _. True" and Q="\<lambda>_ _ _. True"]
+lemmas validI_prefix_closed_T =
+  validI_prefix_closed[where P="\<lambda>_ _. False" and R="\<lambda>_ _. False" and G="\<lambda>_ _. True"
+                         and Q="\<lambda>_ _ _. True"]
 
 lemmas prefix_closedD1 = prefix_closed_def[THEN iffD1, rule_format]
 
